{
 "cells": [
  {
   "cell_type": "markdown",
   "metadata": {},
   "source": [
    "### Fourier transform: Discrete 1D ###\n",
    "\n",
    "Consider a real function $f(x)$ between $0$ and $L$.  We write this as a sum of periodic functions.\n",
    "\n",
    "#### Base defintion ####\n",
    "\n",
    "Start with real variables and positive indicies.\n",
    "\n",
    "\\begin{gather}\n",
    "f(x) = a_0 + \\sum_{n = 1}^{\\infty}\n",
    "\\left[ a_n \\cos \\left(\\frac{2 \\pi n}{L} x\\right) + b_n \\sin \\left(\\frac{2 \\pi n}{L} x\\right) \\right]\n",
    "\\end{gather}\n",
    "\n",
    "Calculations yeild the following.\n",
    "\n",
    "\\begin{gather}\n",
    "a_0 = \\frac{1}{L} \\int_0^L f(x) dx \\\\\n",
    "a_n = \\frac{2}{L} \\int_0^L f(x) \\cos \\left(\\frac{2 \\pi n}{L} x\\right) dx \\\\\n",
    "b_n = \\frac{2}{L} \\int_0^L f(x) \\sin \\left(\\frac{2 \\pi n}{L} x\\right) dx\n",
    "\\end{gather}\n",
    "\n",
    "Note that\n",
    "\n",
    "\\begin{gather}\n",
    "a_{-n} = a_n \\qquad\n",
    "b_{-n} = -b_n\n",
    "\\end{gather}"
   ]
  },
  {
   "cell_type": "markdown",
   "metadata": {},
   "source": [
    "#### First notation update ####\n",
    "\n",
    "Set $k_n = 2 \\pi n / L$, allow $n$ to have integer values, and introduce $a_n$ and $b_n$.  \n",
    "\n",
    "\\begin{gather}\n",
    "f(x) = \\sum_{n = -\\infty}^{\\infty} \\left[ A_n \\cos \\left(k_n x\\right) + B_n \\sin \\left(k_n x\\right) \\right]\n",
    "\\end{gather}\n",
    "\n",
    "Calculations yeild the following.\n",
    "\n",
    "\\begin{gather}\n",
    "A_n = \\frac{1}{L} \\int_0^L f(x) \\cos \\left(k_n x\\right) dx \\\\\n",
    "B_n = \\frac{1}{L} \\int_0^L f(x) \\sin \\left(k_n x\\right) dx\n",
    "\\end{gather}\n",
    "\n",
    "\n",
    "Note that\n",
    "\n",
    "\\begin{gather}\n",
    "A_{-n} = A_n \\qquad\n",
    "B_{-n} = -B_n\n",
    "\\end{gather}\n",
    "\n",
    "Connect this to the old notation.\n",
    "\n",
    "\\begin{gather}\n",
    "a_0 = A_0 \\qquad\n",
    "a_n = 2 A_n \\qquad\n",
    "b_n = 2 B_n\n",
    "\\end{gather}"
   ]
  },
  {
   "cell_type": "markdown",
   "metadata": {},
   "source": [
    "#### Second notation update ####\n",
    "\n",
    "Replace the tigonmetric functions with complex exponentials and introduce the complex quantity $F_n$.\n",
    "\n",
    "\\begin{gather}\n",
    "f(x) = \\sum_{n = -\\infty}^{\\infty} F_n e^{i k_n x}\n",
    "\\end{gather}\n",
    "\n",
    "Calculations yeild the following.\n",
    "\n",
    "\\begin{gather}\n",
    "F_n = \\frac{1}{L} \\int_0^L f(x) e^{-i k_n x} dx\n",
    "\\end{gather}\n",
    "\n",
    "Note that\n",
    "\n",
    "\\begin{gather}\n",
    "F^*_n = F_{-n}\n",
    "\\end{gather}\n",
    "\n",
    "Connect this to the old notation.\n",
    "\n",
    "\\begin{gather}\n",
    "A_n = \\frac{1}{2} (F_n + F^*_n) \\qquad\n",
    "B_n = \\frac{i}{2} (F_n - F^*_n)\n",
    "\\end{gather}\n",
    "\n",
    "\\begin{gather}\n",
    "A_n = \\Re(F_n) \\qquad\n",
    "B_n = -\\Im(F_n)\n",
    "\\end{gather}"
   ]
  },
  {
   "cell_type": "markdown",
   "metadata": {},
   "source": [
    "#### Delta functions ####\n",
    "\n",
    "Consistency leads to the following.\n",
    "\n",
    "\\begin{gather}\n",
    "\\delta(x - x') = \\frac{1}{L} \\sum_{n = -\\infty}^{\\infty} e^{i k_n (x - x')} \\\\\n",
    "\\delta_{n n'} = \\frac{1}{L} \\int_0^L e^{-i (k_n - k_{n'}) x} dx\n",
    "\\end{gather}\n",
    "\n",
    "One can show that $\\delta(-x) = \\delta(x)$ and that $\\delta_{n' n} = \\delta_{n n'}$."
   ]
  },
  {
   "cell_type": "markdown",
   "metadata": {},
   "source": [
    "#### Complex functions ####\n",
    "\n",
    "Consider a complex function $w(x)$ between $0$ and $L$. \n",
    "\n",
    "\\begin{gather}\n",
    "w(x) = u(x) + i v(x)\n",
    "\\end{gather}\n",
    "\n",
    "Define.\n",
    "\n",
    "\\begin{gather}\n",
    "u(x) = \\sum_{n = -\\infty}^{\\infty} U_n e^{i k_n x} \\qquad\n",
    "U_n = \\frac{1}{L} \\int_0^L u(x) e^{-i k_n x} dx \\\\\n",
    "v(x) = \\sum_{n = -\\infty}^{\\infty} V_n e^{i k_n x} \\qquad\n",
    "V_n = \\frac{1}{L} \\int_0^L v(x) e^{-i k_n x} dx \\\\\n",
    "w(x) = \\sum_{n = -\\infty}^{\\infty} W_n e^{i k_n x} \\qquad\n",
    "W_n = \\frac{1}{L} \\int_0^L w(x) e^{-i k_n x} dx\n",
    "\\end{gather}\n",
    "\n",
    "Calculations yeild.\n",
    "\n",
    "\\begin{gather}\n",
    "U_n = \\frac{1}{2}(W_n + W^*_{-n}) \\\\\n",
    "V_n = -\\frac{i}{2}(W_n - W^*_{-n})\n",
    "\\end{gather}\n",
    "\n",
    "Hence, we can store two real functions in the complex quantity $W_n$."
   ]
  },
  {
   "cell_type": "markdown",
   "metadata": {},
   "source": [
    "### Fourier transform: Discrete 2D ###\n",
    "\n",
    "Consider a real function $f(x, y)$ in an $L$ by $L$ square.  Start as before.\n",
    "\n",
    "\\begin{gather}\n",
    "f(x, y) = \\sum_{m = -\\infty}^{\\infty} F_m(y) e^{ i k_m x} \\\\\n",
    "F_m(y) = \\frac{1}{L} \\int_0^L f(x, y) e^{-i k_m x} dx\n",
    "\\end{gather}\n",
    "\n",
    "Now, Foureir expand the complex quantity $F_m(y)$.\n",
    "\n",
    "\\begin{gather}\n",
    "F_m(y) = \\sum_{n = -\\infty}^{\\infty} F_{m n} e^{i k_n y} \\\\\n",
    "F_{m n} = \\frac{1}{L} \\int_0^L F_m(y) e^{- i k_n y} dy\n",
    "\\end{gather}\n",
    "\n",
    "Plug into the previous equations.\n",
    "\n",
    "\\begin{gather}\n",
    "f(x, y) = \\sum_{m = -\\infty}^{\\infty} \\sum_{n = -\\infty}^{\\infty} F_{m n} e^{i (k_m x + k_n y)} \\\\\n",
    "F_{m n} = \\left(\\frac{1}{L}\\right)^2 \\int_0^L \\int_0^L f(x, y) e^{-i \\left(k_m x + k_n y\\right)} dx dy\n",
    "\\end{gather}\n",
    "\n",
    "The generalization to higher dimensions is clear."
   ]
  },
  {
   "cell_type": "markdown",
   "metadata": {},
   "source": [
    "### Fourier Transform: Continuous 1D ###\n",
    "\n",
    "Consider a real function $f(x)$ on the entire real line.  In this case, a different starting notation is better.  First, shift the domain.\n",
    "\n",
    "\\begin{gather}\n",
    "f(x) = \\sum_{n = -\\infty}^{\\infty} F_n e^{i k_n x} \\\\\n",
    "F_n = \\frac{1}{L} \\int_{-L/2}^{L/2} f(x) e^{-i k_n x} dx\n",
    "\\end{gather}\n",
    "\n",
    "Next, define $\\tilde f(k_n) = F_n L$ and $\\Delta k_n = 2 \\pi / L$.\n",
    "\n",
    "\\begin{gather}\n",
    "f(x) = \\frac{1}{2 \\pi} \\sum_{n = -\\infty}^{\\infty} \\tilde f(k_n) e^{  i k_n x} \\Delta k_n \\\\\n",
    "\\tilde f(k_n) = \\int_{-L/2}^{L/2} f(x) e^{- i k_n x} dx\n",
    "\\end{gather}\n",
    "\n",
    "Finally, consider the limit $L \\rightarrow \\infty$ where $k_n \\rightarrow k$. \n",
    "\n",
    "\\begin{gather}\n",
    "f(x) = \\frac{1}{2 \\pi} \\int_{-\\infty}^{\\infty} \\tilde f(k) e^{  i k x} dk \\\\\n",
    "\\tilde f(k) = \\int_{-\\infty}^{\\infty} f(x) e^{- i k x} dx\n",
    "\\end{gather}"
   ]
  },
  {
   "cell_type": "markdown",
   "metadata": {},
   "source": [
    "#### Delta functions ####\n",
    "\n",
    "\n",
    "Consistency leads to the following.\n",
    "\n",
    "\\begin{gather}\n",
    "\\delta(x - x') = \\frac{1}{2 \\pi} \\int_{-\\infty}^{\\infty} e^{i k (x - x')} dk \\\\\n",
    "\\delta(k - k') = \\frac{1}{2 \\pi} \\int_{-\\infty}^{\\infty} e^{- i (k - k') x} dx\n",
    "\\end{gather}\n",
    "\n",
    "The above suggests that $\\delta(-x) = \\delta(x)$.  In general, it can be shown that\n",
    "\n",
    "\\begin{gather}\n",
    "\\delta(a x) = \\frac{1}{\\lvert a \\lvert} \\delta(x)\n",
    "\\end{gather}\n",
    "\n"
   ]
  },
  {
   "cell_type": "markdown",
   "metadata": {},
   "source": [
    "### Towards Green's Functions ###\n",
    "\n",
    "Change to position and time.  Consider a driven simple harmonic oscillator.\n",
    "\n",
    "\\begin{gather}\n",
    "\\bigg( \\frac{d^2}{d t^2} + \\omega_0^2 \\bigg) x(t) = \\frac{1}{m} f(t)\n",
    "\\end{gather}\n",
    "\n",
    "For the discrete case, substitue the expression for $x(t)$ into the differential equation.  Solve for $X_n$ by multiplying by $e^{-i \\omega'_n t}$ and integrating with respect to $t$.  Note the delta function and change from $\\omega'_n$ to $\\omega_n$ and $t$ to $t'$.  Solve for $x(t)$ by multiply by $e^{i \\omega_n t}/T$ and summing with respect to $n$.  The solution is written in terms of a Green's function.\n",
    "\n",
    "\\begin{gather}\n",
    "x(t) = \\int_0^T G(t, t') \\frac{1}{m} f(t') dt' \\\\\n",
    "G(t, t') = \\frac{1}{T} \\sum_{n = -\\infty}^{\\infty} \\frac{1}{\\omega_0^2 - \\omega_n^2} e^{i \\omega_n (t - t')}\n",
    "\\end{gather}\n",
    "\n",
    "For the continuous case, substitue the expression for $x(t)$ into the differential equation and solve for $\\tilde x(\\omega)$ by multiplying by $e^{-i \\omega' t}$ and integrating with respect to $t$.  Note the delta function and change from $\\omega'$ to $\\omega$ and $t$ to $t'$. Solve for $x(t)$ by multiply by $e^{i \\omega t}/2\\pi$ and integrating with respect to $\\omega$.  The solution is written in terms of a Green's function.\n",
    "\n",
    "\\begin{gather}\n",
    "x(t) = \\int_{-\\infty}^\\infty G(t, t') \\frac{1}{m} f(t') dt' \\\\\n",
    "G(t, t') = \\frac{1}{2 \\pi} \n",
    "\\int_{-\\infty}^\\infty \\frac{1}{\\omega_0^2 - \\omega^2} e^{i \\omega (t - t')} d\\omega\n",
    "\\end{gather}\n",
    "\n",
    "In both cases, $G(t, t') = G(t', t)$, $G^*(t, t') = G(t, t')$, and\n",
    "\n",
    "\\begin{gather}\n",
    "\\bigg( \\frac{d^2}{d t^2} + \\omega_0^2 \\bigg) G(t, t') = \\delta(t - t')\n",
    "\\end{gather}"
   ]
  },
  {
   "cell_type": "markdown",
   "metadata": {},
   "source": [
    "#### More general Green's functions ####\n",
    "\n",
    "Consider a linear differential operator $L$, which we assume is real.  Our goal is to find solutions to the equation\n",
    "\n",
    "\\begin{gather}\n",
    "L x(t) = f(t)\n",
    "\\end{gather}\n",
    "\n",
    "Assume that we can find some orthogonal solutions $u_n(t)$ to the homogeneous equation with eigenvalues $\\lambda_n$.\n",
    "\n",
    "\\begin{gather}\n",
    "L u_n(t) = \\lambda_n u_n(t) \\qquad\n",
    "L u^*_n(t) = \\lambda^*_n u^*_n(t)\n",
    "\\end{gather}\n",
    "\n",
    "\\begin{gather}\n",
    "\\delta(t - t') = \\frac{1}{T} \\sum_{n = -\\infty}^{\\infty} u_n(t) u^*_n(t') \\\\\n",
    "\\delta_{n n'} = \\frac{1}{T} \\int_0^T u_n(t) u^*_{n'}(t) dt\n",
    "\\end{gather}"
   ]
  },
  {
   "cell_type": "markdown",
   "metadata": {},
   "source": [
    "Also assume\n",
    "\n",
    "\\begin{gather}\n",
    "x(t) = \\sum_{n = -\\infty}^\\infty X_n u_n(t)\n",
    "\\end{gather}\n",
    "\n",
    "Calculations yield.\n",
    "\n",
    "\\begin{gather}\n",
    "X_n = \\frac{1}{T} \\int_0^T x(t) u^*_n(t) dt\n",
    "\\end{gather}"
   ]
  },
  {
   "cell_type": "markdown",
   "metadata": {},
   "source": [
    "\\begin{gather}\n",
    "x(t) = \\int_0^T G(t, t') f(t') dt' \\\\\n",
    "G(t, t') = \\frac{1}{T} \\sum_{n = -\\infty}^{\\infty} \\frac{1}{\\lambda_n} u(t)_n u^*_n(t')\n",
    "\\end{gather}"
   ]
  },
  {
   "cell_type": "markdown",
   "metadata": {},
   "source": [
    "### Matrix albegra ###\n",
    "\n",
    "Begin the ping-pong notation.  Both have their merrits and feed on each other.  Lanzchos is lucid, but not a notation snob.  It's not great.  Perhaps it's the writing and publishing process.  Consider the square matrix $A$ and row vectors $x$ and $b$ that satisfy\n",
    "\n",
    "\\begin{gather}\n",
    "\\sum_n A_{m n} x_n = b_m\n",
    "\\qquad \\Rightarrow \\qquad\n",
    "A x = b\n",
    "\\end{gather}\n",
    "\n",
    "Define eigen values $\\lambda^{(l)}$ and eigen vectors $u^{(l)}$ stored in rows such that\n",
    "\n",
    "\\begin{gather}\n",
    "\\sum_n A_{m n} u^{(l)}_n = \\lambda^{(l)} u^{(l)}_m\n",
    "\\qquad \\Rightarrow \\qquad\n",
    "A u^{(l)} = \\lambda^{(l)} u^{(l)}\n",
    "\\end{gather}\n",
    "\n",
    "\\begin{gather}\n",
    "\\sum_n A^T_{m n} v^{(l)}_n = \\lambda^{(l)} v^{(l)}_m\n",
    "\\qquad \\Rightarrow \\qquad\n",
    "A^T v^{(l)} = \\lambda^{(l)} v^{(l)}\n",
    "\\end{gather}\n",
    "\n",
    "Define $U_{n l} = u^{(l)}_n$, $V_{n l} = v^{(l)}_n$, and $\\Lambda_{n l} = \\delta_{n l} \\lambda^{(l)}$.\n",
    "\n",
    "\\begin{gather}\n",
    "\\sum_n A_{m n} U_{n l} = \\sum_n U_{m n} \\Lambda_{n l}\n",
    "\\qquad \\Rightarrow \\qquad\n",
    "A U = U \\Lambda\n",
    "\\end{gather}\n",
    "\n",
    "\\begin{gather}\n",
    "\\sum_n A^T_{m n} V_{n l} = \\sum_n V_{m n} \\Lambda_{n l}\n",
    "\\qquad \\Rightarrow \\qquad\n",
    "A^T V = V \\Lambda\n",
    "\\end{gather}"
   ]
  },
  {
   "cell_type": "markdown",
   "metadata": {},
   "source": [
    "Take the transpose of the second equation.  Pre-multiply the first by $V^T$ and post multiply the second by $U$.\n",
    "\n",
    "\\begin{gather}\n",
    "A U = U \\Lambda\n",
    "\\qquad \\Rightarrow \\qquad\n",
    "V^T A U = V^T U \\Lambda\n",
    "\\end{gather}\n",
    "\n",
    "\\begin{gather}\n",
    "V^T A = \\Lambda V^T\n",
    "\\qquad \\Rightarrow \\qquad\n",
    "V^T A U = \\Lambda V^T U\n",
    "\\end{gather}\n",
    "\n",
    "Define $W = V^T U$ and subtract the equations.\n",
    "\n",
    "\\begin{gather}\n",
    "W \\Lambda - \\Lambda W = 0\n",
    "\\qquad \\Rightarrow \\qquad\n",
    "(\\lambda^{(m)} - \\lambda^{(n)}) W_{m n} = 0\n",
    "\\end{gather}\n",
    "\n",
    "This means $W_{m n} = \\delta_{m n} w^{(n)}$ is a diagonal matrix.\n",
    "\n",
    "\\begin{gather}\n",
    "U^T V = W\n",
    "\\qquad \\Rightarrow \\qquad\n",
    "u^{(m)} \\cdot v^{(n)} = \\delta_{m n} w^{(n)}\n",
    "\\end{gather}\n",
    "\n",
    "We can rescale either $u^{(m)}$ or $v^{(n)}$ such that\n",
    "\n",
    "\\begin{gather}\n",
    "u^{(m)} \\cdot v^{(n)} = \\delta_{m n}\n",
    "\\qquad \\Rightarrow \\qquad\n",
    "U^T V = V^T U = I\n",
    "\\end{gather}\n",
    "\n",
    "It follows that\n",
    "\n",
    "\\begin{gather}\n",
    "U^{-1} = V^T \\qquad\n",
    "V^{-1} = U^T \\qquad\n",
    "(U^T)^{-1} = V \\qquad\n",
    "(V^T)^{-1} = U\n",
    "\\end{gather}\n",
    "\n",
    "\\begin{gather}\n",
    "(U^{-1})^T = V \\qquad\n",
    "(V^{-1})^T = U\n",
    "\\end{gather}\n",
    "\n",
    "and that\n",
    "\n",
    "\\begin{gather}\n",
    "A = U \\Lambda V^T \\qquad\n",
    "A^T = V \\Lambda U^T\n",
    "\\end{gather}\n",
    "\n",
    "Define $(\\Lambda^{-1})_{m n} = \\delta_{m n} (\\lambda^{-1})^{(n)}$.  There are also expressions for inverses.\n",
    "\n",
    "\\begin{gather}\n",
    "A^{-1} = U \\Lambda^{-1} V^T \\qquad\n",
    "(A^T)^{-1} = V \\Lambda^{-1} U^T\n",
    "\\end{gather}\n",
    "\n",
    "And return to the eigenvalues.\n",
    "\n",
    "\\begin{gather}\n",
    "A^{-1} U = U \\Lambda^{-1} \\qquad\n",
    "(A^T)^{-1} V = V \\Lambda^{-1}\n",
    "\\end{gather}"
   ]
  },
  {
   "cell_type": "markdown",
   "metadata": {},
   "source": [
    "### Conic sections ###\n",
    "\n",
    "In general, conic section are written as\n",
    "\n",
    "\\begin{gather}\n",
    "\\sum_n \\lambda^{(n)} x_n^2 = 1\n",
    "\\end{gather}\n",
    "\n",
    "With rotated and scaled coordinates, we have\n",
    "\n",
    "\\begin{gather}\n",
    "\\sum_{m n} A_{m n} x_m x_n = 1\n",
    "\\qquad \\Rightarrow \\qquad\n",
    "x^T A x = 1\n",
    "\\end{gather}\n",
    "\n",
    "Also, one can show that we get the same conic section with\n",
    "\n",
    "\\begin{gather}\n",
    "\\sum_{m n} \\frac{1}{2} A_{m n} (x_m x_n + x_n x_m)\n",
    "= \\sum_{m n} \\frac{1}{2} (A_{m n} + A^T_{m n}) x_m x_n\n",
    "=  1\n",
    "\\end{gather}\n",
    "\n",
    "Hence, it make sense to say the surface is defined as\n",
    "\n",
    "\\begin{gather}\n",
    "\\sum_{m n} S_{m n} x_m x_n = 1\n",
    "\\qquad \\Rightarrow \\qquad\n",
    "x^T S x = 1\n",
    "\\end{gather}\n",
    "\n",
    "where we have the symmetric tensor $S^T = S$."
   ]
  },
  {
   "cell_type": "markdown",
   "metadata": {},
   "source": [
    "### New coordinates ###\n",
    "\n",
    "The coordinate system is $x = \\sum_n x_n e^{(n)}$.  Choose a new coordinate system where $x = \\sum_n \\bar x_n u^{(n)}$ with basis vectors $u^{(n)}$ oriented along the principle axes.  With calculus, it is clear one needs\n",
    "\n",
    "\\begin{gather}\n",
    "S u^{(l)} = \\lambda^{(l)} u^{(l)}\n",
    "\\qquad \\Rightarrow \\qquad\n",
    "S U = U \\Lambda \n",
    "\\end{gather}\n",
    "\n",
    "Since $S^T = S$, we have $U^{-1} = U^T$ and we can scale such that\n",
    "\n",
    "\\begin{gather}\n",
    "U^T U = I\n",
    "\\qquad \\Rightarrow \\qquad\n",
    "u^{(m)} \\cdot u^{(l)} = \\delta_{m l}\n",
    "\\end{gather}\n",
    "\n",
    "Hence, the $u^{(l)}$ form an orthogonal coordinate systme.  Since $S = U \\Lambda U^T$, we have\n",
    "\n",
    "\\begin{gather}\n",
    "\\bar x^T \\Lambda \\bar x  = 1\n",
    "\\qquad \\Rightarrow \\qquad\n",
    "\\sum_m \\lambda^{(m)} \\bar x_m^2 = 1\n",
    "\\end{gather}\n",
    "\n",
    "where\n",
    "\n",
    "\\begin{gather}\n",
    "\\bar x = U^T x\n",
    "\\qquad \\Rightarrow \\qquad\n",
    "\\bar x_m = u^{(m)} \\cdot x\n",
    "\\end{gather}\n",
    "\n",
    "\\begin{gather}\n",
    "x = U \\bar x\n",
    "\\qquad \\Rightarrow \\qquad\n",
    "x = \\sum_n \\bar x_n u^{(n)}\n",
    "\\end{gather}"
   ]
  },
  {
   "cell_type": "markdown",
   "metadata": {},
   "source": [
    "#### Complex ####\n",
    "\n",
    "Let us consider the reality of $\\lambda^{(l)}$.  Along with being symmetric, $S$ is also real.  Define $S^\\dagger = S^{* T}$.\n",
    "\n",
    "\\begin{gather}\n",
    "S U = U \\Lambda\n",
    "\\qquad \\Rightarrow \\qquad\n",
    "U^\\dagger S U = U^\\dagger U \\Lambda\n",
    "\\end{gather}\n",
    "\n",
    "\\begin{gather}\n",
    "U^\\dagger S = \\Lambda^* U^\\dagger\n",
    "\\qquad \\Rightarrow \\qquad\n",
    "U^\\dagger S U = \\Lambda^* U^\\dagger U\n",
    "\\end{gather}\n",
    "\n",
    "Subtracting the equations and noting that $\\Lambda$ is diagonal and commutes, we have $\\Lambda^* - \\Lambda = 0$.  Hence, the eigenvalues are real.  Note that this arguement holds for any Hermitian matrix $S^\\dagger = S$, which is not by itself real or symmetric.  That is, the eigenvalues for any Hermitian matrix are real.\n"
   ]
  },
  {
   "cell_type": "markdown",
   "metadata": {},
   "source": [
    "#### Coordinates 2: Slant ####\n",
    "\n",
    "Now $u_n$ are not an orthogonal basis but they are linearly independent.  We need an adjoint basis $v_n$ too.  Write\n",
    "\n",
    "\\begin{gather}\n",
    "r = \\sum_n x_n u^{(n)}  = \\sum_n y_n v^{(n)}\n",
    "\\qquad \\Rightarrow \\qquad\n",
    "r = U x = V y\n",
    "\\end{gather}\n",
    "\n",
    "where\n",
    "\n",
    "\\begin{gather}\n",
    "u^{(m)} \\cdot v^{(n)} = \\delta_{m n}\n",
    "\\qquad \\Rightarrow \\qquad\n",
    "U^T V = V^T U = I\n",
    "\\end{gather}\n",
    "\n",
    "Say that we have a different vector\n",
    "\n",
    "\\begin{gather}\n",
    "r' = \\sum_n x_n' u^{(n)}  = \\sum_n y_n' v^{(n)}\n",
    "\\qquad \\Rightarrow \\qquad\n",
    "r' = U x' = V y'\n",
    "\\end{gather}\n",
    "\n",
    "The dot product\n",
    "\n",
    "\\begin{gather}\n",
    "r' \\cdot r = x' \\cdot y = x \\cdot y'\n",
    "\\end{gather}"
   ]
  },
  {
   "cell_type": "markdown",
   "metadata": {},
   "source": [
    "\\begin{gather}\n",
    "\\bar u^{(m)} = \\sum_n P_{m n} u^{(n)}\n",
    "\\qquad \\Rightarrow \\qquad\n",
    "\\bar U = U P^T\n",
    "\\end{gather}\n",
    "\n",
    "\\begin{gather}\n",
    "\\bar v^{(m)} = \\sum_n Q_{m n} v^{(n)}\n",
    "\\qquad \\Rightarrow \\qquad\n",
    "\\bar V = V Q^T\n",
    "\\end{gather}\n",
    "\n",
    "\\begin{gather}\n",
    "\\bar U^T \\bar V = P U^T V Q^T = P Q^T = I\n",
    "\\end{gather}"
   ]
  },
  {
   "cell_type": "markdown",
   "metadata": {},
   "source": [
    "\\begin{gather}\n",
    "r = \\bar U \\bar x = \\bar V \\bar y\n",
    "\\end{gather}\n",
    "\n",
    "\\begin{gather}\n",
    "r = U P^T \\bar x = V Q^T \\bar y\n",
    "\\end{gather}"
   ]
  },
  {
   "cell_type": "code",
   "execution_count": null,
   "metadata": {
    "collapsed": true
   },
   "outputs": [],
   "source": []
  }
 ],
 "metadata": {
  "kernelspec": {
   "display_name": "Python 3",
   "language": "python",
   "name": "python3"
  },
  "language_info": {
   "codemirror_mode": {
    "name": "ipython",
    "version": 3
   },
   "file_extension": ".py",
   "mimetype": "text/x-python",
   "name": "python",
   "nbconvert_exporter": "python",
   "pygments_lexer": "ipython3",
   "version": "3.7.3"
  }
 },
 "nbformat": 4,
 "nbformat_minor": 2
}
