{
 "cells": [
  {
   "cell_type": "markdown",
   "metadata": {
    "deletable": true,
    "editable": true
   },
   "source": [
    "<h2>Fourier transform: Discrete 1D</h2>\n",
    "\n",
    "<p>Consider a real function $f(x)$ that is periodic between $0$ and $L$.</p>\n",
    "\n",
    "<h3>The base defintion</h3>\n",
    "\n",
    "<p>The first definition has all real functions and positive indicies.\n",
    "\n",
    "$$ f(x) = A_0 + \\sum_{n = 1}^{N} \\left[\n",
    "          A_n \\cos \\left(\\frac{2 \\pi n}{L} x\\right)\n",
    "        + B_n \\sin \\left(\\frac{2 \\pi n}{L} x\\right) \n",
    "   \\right] $$\n",
    "\n",
    "$$ A_0 = \\frac{1}{L} \\int_0^L f(x) dx $$\n",
    "\n",
    "$$ A_n = \\frac{2}{L} \\int_0^L f(x) \\cos \\left(\\frac{2 \\pi n}{L} x\\right) dx $$\n",
    "\n",
    "$$ B_n = \\frac{2}{L} \\int_0^L f(x) \\sin \\left(\\frac{2 \\pi n}{L} x\\right) dx $$</p>\n",
    "\n",
    "<h3>The first notational update</h3>\n",
    "\n",
    "<p>We can compacitfy things up by allowing $n$ to be negative and setting $k_n = 2 \\pi n / L$.  \n",
    "\n",
    "$$ f(x) = \\sum_{n = -N}^{N} \\left[\n",
    "          a_n \\cos \\left(k_n x\\right)\n",
    "        + b_n \\sin \\left(k_n x\\right) \n",
    "   \\right] $$\n",
    "\n",
    "$$ a_n = \\frac{1}{L} \\int_0^L f(x) \\cos \\left(k_n x\\right) dx $$\n",
    "\n",
    "$$ b_n = \\frac{1}{L} \\int_0^L f(x) \\sin \\left(k_n x\\right) dx $$\n",
    "\n",
    "We can connect this to the older notation.\n",
    "\n",
    "$$ A_0 = a_0 $$\n",
    "\n",
    "$$ A_n = 2 a_n, \\quad n > 1 $$\n",
    "\n",
    "$$ B_n = 2 b_n, \\quad n > 1 $$\n",
    "\n",
    "Also, note the following.\n",
    "\n",
    "$$ a_{-n} = a_n $$\n",
    "\n",
    "$$ b_{-n} = - b_n $$\n",
    "\n",
    "</p>"
   ]
  },
  {
   "cell_type": "markdown",
   "metadata": {
    "deletable": true,
    "editable": true
   },
   "source": [
    "<h3>The second notational update</h3>\n",
    "\n",
    "<p>Let us write the trig functions as complex exponentials and introduce new variables.\n",
    "\n",
    "$$ c_n    = a_n - i b_n $$\n",
    "\n",
    "$$ c_{-n} = a_n + i b_n $$\n",
    "\n",
    "\n",
    "This allows us to write the following.\n",
    "\n",
    "$$ f(x) = \\sum_{n = -N}^{N} c_n    e^{  i k_n x} $$\n",
    "\n",
    "$$ c_n = \\frac{1}{L} \\int_0^L f(x) e^{- i k_n x} dx $$\n",
    "\n",
    "We can connect to the origionla notation.\n",
    "\n",
    "$$ A_0 = c_0 $$\n",
    "\n",
    "$$ A_n = c_n + c_{-n}, \\quad n > 1 $$\n",
    "\n",
    "$$ B_n = i (c_n - c_{-n}), \\quad n > 1 $$\n",
    "\n",
    "</p>"
   ]
  },
  {
   "cell_type": "markdown",
   "metadata": {
    "deletable": true,
    "editable": true
   },
   "source": [
    "<h3>Delta functions</h3>\n",
    "\n",
    "<p>Using a circular arguemtents we discover delta functions.  The first delta function is implied by the following.\n",
    "\n",
    "$$ f(x) = \\int_0^L f(x') \\frac{1}{L} \\sum_{n = -\\infty}^{\\infty} e^{i k_n (x - x')} dx' $$\n",
    "\n",
    "$$ \\delta(x - x') = \\frac{1}{L} \\sum_{n = -\\infty}^{\\infty} e^{i k_n (x - x')} $$\n",
    "\n",
    "The second delta functions is implied in a similar way.\n",
    "\n",
    "$$ c_n = \\sum_{n' = -\\infty}^{\\infty} c_{n'} \\frac{1}{L} \\int_0^L e^{-i (k_n - k_{n'}) x} dx $$\n",
    "\n",
    "$$ \\delta_{n n'} = \\frac{1}{L} \\int_0^L e^{-i (k_n - k_{n'}) x} dx $$\n",
    "\n",
    "</p>"
   ]
  },
  {
   "cell_type": "markdown",
   "metadata": {
    "deletable": true,
    "editable": true
   },
   "source": [
    "<h2>Fourier transform: Discrete 2D</h2>\n",
    "\n",
    "<p>Consider a two dimentional functions.  We can start as before.\n",
    "\n",
    "$$ f(x, y) = \\sum_{n = -N}^{N} c_n(y)    e^{  i k_n x} $$\n",
    "\n",
    "$$ c_n(y) = \\frac{1}{L} \\int_0^L f(x, y) e^{- i k_n x} dx $$\n",
    "\n",
    "Now, Foureir expand $c_n(y)$.\n",
    "\n",
    "$$ c_n(y) = \\sum_{m = -M}^{M} c_{nm} e^{i k_m y} $$\n",
    "\n",
    "$$ c_{nm} = \\frac{1}{L} \\int_0^L c_n(y) e^{- i k_m y} dy $$\n",
    "\n",
    "Plugging back into the first equations we have the following symmetric relationship.\n",
    "\n",
    "$$ f(x, y) = \\sum_{n = -N}^{N} \\sum_{m = -M}^{M} c_{nm} \n",
    "             e^{i (k_n x + k_m y)} $$\n",
    "\n",
    "$$ c_{nm} = \\left(\\frac{1}{L}\\right)^2\n",
    "            \\int_0^L \\int_0^L f(x, y)\n",
    "            e^{ -i \\left(k_n x + k_m y\\right)} dx dy $$\n",
    "</p>"
   ]
  },
  {
   "cell_type": "markdown",
   "metadata": {
    "deletable": true,
    "editable": true
   },
   "source": [
    "<h2>Fourier Transform: Continuous 1D</h2>\n",
    "\n",
    "<p>Considering a continuous limit, we see that a different starting notation would have been better.  Hence, we introduce $c_n = \\frac{1}{L} c(k_n)$.  With this change in notation, noting $\\Delta k_n = \\frac{2 \\pi}{L}$, and a shift in the integration limits we have the following.\n",
    "\n",
    "$$ f(x) = \\frac{1}{2 \\pi} \\sum_{n = -\\infty}^{\\infty} c(k_n) e^{ i k_n x} \\Delta k_n $$\n",
    "\n",
    "$$ c(k_n) = \\int_{-L/2}^{L/2} f(x) e^{- i k_n x} dx $$\n",
    "\n",
    "Now, we take the limit as $L$ goes to $\\infty$ as $k_n$ goes to $k$.\n",
    "\n",
    "$$ f(x) = \\frac{1}{2 \\pi} \\int_{-\\infty}^{\\infty} c(k) e^{ i k x} dk $$\n",
    "\n",
    "$$ c(k) = \\int_{-\\infty}^{\\infty} f(x) e^{- i k x} dx $$\n",
    "\n",
    "</p>"
   ]
  },
  {
   "cell_type": "markdown",
   "metadata": {
    "deletable": true,
    "editable": true
   },
   "source": [
    "<h3>The wave equation</h3>\n",
    "\n",
    "<p> Consider the wave equation\n",
    "\n",
    "$$ \\frac{\\partial^2 \\phi}{\\partial t^2} = c^2 \\frac{\\partial^2 \\phi}{\\partial x^2} $$\n",
    "\n",
    "where\n",
    "\n",
    "$$ \\phi(x,0) = \\phi_0(x) $$\n",
    "$$ \\dot\\phi(x, 0) = \\pi_0(x) $$\n",
    "\n",
    "Let us take the Fourier transform of the equation.\n",
    "\n",
    "$$ \\int_{-\\infty}^\\infty e^{-i k x}\n",
    "   \\frac{\\partial^2 \\phi}{\\partial t^2} dx\n",
    " = \\int_{-\\infty}^\\infty e^{-i k x} c^2 \\frac{\\partial^2 \\phi}{\\partial x^2} dx $$\n",
    "\n",
    "With some algebra, integration by parts, and assumptions about the function at infinity we get the following.\n",
    "\n",
    "$$ \\frac{\\partial^2}{\\partial t^2} \\int_{-\\infty}^\\infty\n",
    "   \\phi(x, t) e^{-i k x} dx\n",
    " = -c^2 k^2 \\int_{-\\infty}^\\infty \\phi(x, t) e^{-i k x} dx $$\n",
    "\n",
    "Now define the transform where there is a change in notation from before.\n",
    "\n",
    "$$ \\phi(x, t) = \\frac{1}{2 \\pi} \\int_{-\\infty}^\\infty \\hat\\phi(k, t) e^{i k x} dk $$\n",
    "\n",
    "$$ \\hat\\phi(k, t) = \\int_{-\\infty}^\\infty \\phi(x, t) e^{-i k x} dx $$\n",
    "\n",
    "The wave equation then says\n",
    "\n",
    "$$ \\frac{d^2 \\hat\\phi}{d t^2} = -c^2 k^2 \\hat\\phi $$\n",
    "\n",
    "This has the solution\n",
    "\n",
    "$$ \\hat\\phi(k,t) = \\hat f(k) e^{i c k t} + \\hat g(k) e^{-i c k t} $$\n",
    "\n",
    "so\n",
    "\n",
    "$$ \\phi(x, t) = \\frac{1}{2 \\pi} \\int_{-\\infty}^\\infty \\left[\n",
    "   \\hat f(k) e^{i k (x + c t)} + \\hat g(k) e^{i k (x - c t)} \\right] dk $$\n",
    "\n",
    "This leads to a classical result, which we will not use later.\n",
    "\n",
    "$$ \\phi(x, t) = f(x + c t) + g(x - c t) $$\n",
    "\n",
    "Now let us consider the initial conditions.  With some algebra you can show the following.\n",
    "\n",
    "$$ \\hat f(k) = \\frac{1}{2} \\left(\\hat\\phi_0(k) + \\frac{1}{i c k}\\hat\\pi_0(k) \\right) $$\n",
    "\n",
    "$$ \\hat g(k) = \\frac{1}{2} \\left(\\hat\\phi_0(k) - \\frac{1}{i c k}\\hat\\pi_0(k) \\right) $$\n",
    "\n",
    "The resulting equation is fairly long so let us break it into two parts.\n",
    "\n",
    "$$ \\phi(x, t) = \\phi_1(x, t) + \\phi_2(x, t) $$\n",
    "\n",
    "The first party is easy.\n",
    "\n",
    "$$ \\phi_1 (x, t) = \\frac{1}{2 \\pi} \\int_{-\\infty}^\\infty \\frac{1}{2} \\left[\n",
    "   \\hat\\phi_0(k) e^{i k (x + c t)}\n",
    " + \\hat\\phi_0(k) e^{i k (x - c t)} \\right] dk $$\n",
    "\n",
    "The second part is more complicated and involves some integation by parts.\n",
    "\n",
    "$$ \\phi_2(x, t) = \\frac{1}{2 \\pi} \\int_{-\\infty}^\\infty \\frac{1}{2} \\left[\n",
    "   \\frac{1}{i c k}\\hat\\pi_0(k) e^{i k (x + c t)}\n",
    "  -\\frac{1}{i c k}\\hat\\pi_0(k) e^{i k (x - c t)}\n",
    "   \\right] dk $$\n",
    "   \n",
    "$$ \\phi_2(x, t) = \\frac{1}{2 \\pi} \\int_{-\\infty}^\\infty \\frac{1}{2} \n",
    "   \\int_0^{t}\\left[\n",
    "   \\hat\\pi_0(k) e^{i k (x + c t')}\n",
    "  +\\hat\\pi_0(k) e^{i k (x - c t')}\n",
    "   \\right] dt' dk $$\n",
    "\n",
    "The results are the follwoing.\n",
    "\n",
    "$$ \\phi_1 (x, t) = \\frac{1}{2} \\left[\n",
    "   \\phi_0(x + c t) + \\phi_0(x - c t) \\right] $$ \n",
    "   \n",
    "$$ \\phi_2(x, t) = \\frac{1}{2} \\int_0^t \\left[\n",
    "   \\pi_0(x + c t') + \\pi_0(x - c t') \\right] dt' $$\n",
    "\n",
    "Finally, we arrive at the d'Alembera solution by rewriting the second piece.\n",
    "\n",
    "$$ \\phi_2(x, t) = \\frac{1}{2 c}\n",
    "   \\int_{x - c t}^{x + c t} \\pi_0(\\xi) d\\xi $$\n",
    "\n",
    "Here is the classical result.\n",
    "\n",
    "$$ \\phi(x, t) = \\frac{1}{2} \\left[\n",
    "   \\phi_0(x + c t) + \\phi_0(x - c t) \\right]\n",
    " + \\frac{1}{2 c}\n",
    "   \\int_{x - c t}^{x + c t} \\pi_0(\\xi) d\\xi $$\n",
    " \n",
    "</p>"
   ]
  },
  {
   "cell_type": "markdown",
   "metadata": {},
   "source": [
    "<h2>Wave Equation: Discrete 2D</h2>\n",
    "\n",
    "$$ f(x, y, t) = \\sum_{n = -N}^{N} \\sum_{m = -M}^{M} c_{nm}(t) \n",
    "             e^{i (k_n x + k_m y)} $$\n",
    "\n",
    "$$ c_{nm}(t) = \\left(\\frac{1}{L}\\right)^2\n",
    "            \\int_0^L \\int_0^L f(x, y, t)\n",
    "            e^{ -i \\left(k_n x + k_m y\\right)} dx dy $$\n",
    "\n",
    "$$ \\frac{\\partial^2 f}{\\partial x^2} + \\frac{\\partial^2 f}{\\partial y^2} - \\frac{1}{c^2} \\frac{\\partial^2 f}{\\partial t^2} = 0 $$"
   ]
  },
  {
   "cell_type": "markdown",
   "metadata": {},
   "source": [
    "Plugging into the wave equation we get the following.\n",
    "\n",
    "$$ \\sum_{n = -N}^{N} \\sum_{m = -M}^{M} \\left[ \n",
    "-(k_n^2 + k_m^2) c_{nm} - \\frac{1}{c^2} \\frac{d^2 c_{nm}}{d t^2} \\right] e^{i (k_n x + k_m y)} = 0 $$ \n",
    "\n",
    "Assuming periodic boundary conditions.\n",
    "\n",
    "$$ \\frac{d^2 c_{nm}}{d t^2} = -c^2 (k_n^2 + k_m^2) c_{nm} $$ \n",
    "\n",
    "$$ \\frac{d^2 c_{nm}}{d t^2} = - \\omega^2_{nm} c_{nm} $$\n",
    "\n",
    "$$ c_{nm} = a_{nm} e^{i w_{nm} t} + b_{nm} e^{-i w_{nm} t} $$\n",
    "\n",
    "$$ f(x, y, t) = \\sum_{n = -N}^{N} \\sum_{m = -M}^{M} (a_{nm} e^{i w_{nm} t} + b_{nm} e^{-i w_{nm} t}) e^{i (k_n x + k_m y)} $$\n",
    "\n",
    "\n",
    "$$ f(x, y, t) = \\sum_{n = -N}^{N} \\sum_{m = -M}^{M}\n",
    "  \\left[ a_{nm} e^{i (k_n x + k_m y + w_{nm} t)}\n",
    " + b_{nm} e^{i (k_n x + k_m y - w_{nm} t)} \\right] $$\n",
    " \n",
    "$$ f_0 = \\sum_{n = -N}^{N} \\sum_{m = -M}^{M}\n",
    "  \\left[ a_{nm} + b_{nm} \\right] e^{i (k_n x + k_m y)} $$\n",
    "\n",
    "$$ \\dot f_0 = \\sum_{n = -N}^{N} \\sum_{m = -M}^{M}\n",
    " i \\omega_{nm} \\left[ a_{nm} - b_{nm} \\right] e^{i (k_n x + k_m y)}$$\n",
    " \n",
    "$$ a_{nm} + b_{nm} \n",
    " = \\left(\\frac{1}{L}\\right)^2 \\int_0^L \\int_0^L\n",
    "   f_0 (x, y) e^{-i (k_n x + k_m y)} dx dy $$\n",
    "\n",
    "$$ a_{nm} - b_{nm} \n",
    " = \\left(\\frac{1}{L}\\right)^2 \\int_0^L \\int_0^L\n",
    "   \\frac{1}{i \\omega_{nm}} \\dot f_0 (x, y)\n",
    "   e^{-i (k_n x + k_m y)} dx dy $$\n",
    "   \n",
    "$$ a_{nm} = \\frac{1}{2}\\left(\\frac{1}{L}\\right)^2 \\int_0^L \\int_0^L\n",
    "   \\left[ f_0 (x, y) + \\frac{1}{i \\omega_{nm}} \\dot f_0 (x, y) \\right]\n",
    "   e^{-i (k_n x + k_m y)} dx dy $$   \n",
    "   \n",
    "$$ b_{nm} = \\frac{1}{2}\\left(\\frac{1}{L}\\right)^2 \\int_0^L \\int_0^L\n",
    "   \\left[ f_0 (x, y) - \\frac{1}{i \\omega_{nm}} \\dot f_0 (x, y) \\right]\n",
    "   e^{-i (k_n x + k_m y)} dx dy $$"
   ]
  },
  {
   "cell_type": "markdown",
   "metadata": {
    "collapsed": true
   },
   "source": [
    "<h3>Rethink</h3>\n",
    "\n",
    "$$ f(x, y, t) = \\sum_{n = -N}^{N} \\sum_{m = -M}^{M}\n",
    "  \\left[ a_{nm} e^{i (k_n x + k_m y + w_{nm} t)}\n",
    " + a^*_{nm} e^{-i (k_n x + k_m y + w_{nm} t)} \\right] $$\n",
    "\n",
    "$$ a_{nm} = \\frac{1}{2}\\left(\\frac{1}{L}\\right)^2 \\int_0^L \\int_0^L\n",
    "   \\left[ f_0 (x, y) + \\frac{1}{i \\omega_{nm}} \\dot f_0 (x, y) \\right]\n",
    "   e^{-i (k_n x + k_m y)} dx dy $$   \n",
    "   \n",
    "$$ a^*_{nm} = \\frac{1}{2}\\left(\\frac{1}{L}\\right)^2 \\int_0^L \\int_0^L\n",
    "   \\left[ f_0 (x, y) - \\frac{1}{i \\omega_{nm}} \\dot f_0 (x, y) \\right]\n",
    "   e^{i (k_n x + k_m y)} dx dy $$"
   ]
  },
  {
   "cell_type": "markdown",
   "metadata": {},
   "source": [
    "<h3>Rethink Again</h3>\n",
    "\n",
    "$$ f(x, y, t) = \\sum_{n = -N}^{N} \\sum_{m = -M}^{M}\n",
    "  \\left[ c_{nm} \\cos(\\omega_{nm} t)\n",
    "  + \\frac{\\dot c_{nm}}{\\omega_{nm}} \\sin(\\omega_{nm} t) \n",
    "  \\right ]e^{i (k_n x + k_m y)} $$\n",
    "\n",
    "$$ \\omega_{nm} = c \\sqrt{k_n^2 + k_m^2} $$\n",
    "\n",
    "$$ c_{nm} = \\left(\\frac{1}{L}\\right)^2\n",
    "  \\int_0^L \\int_0^L f(x, y, 0)\n",
    "  e^{ -i \\left(k_n x + k_m y\\right)} dx dy $$\n",
    "  \n",
    "$$ \\dot c_{nm} = \\left(\\frac{1}{L}\\right)^2\n",
    "  \\int_0^L \\int_0^L \\dot f(x, y, 0)\n",
    "  e^{ -i \\left(k_n x + k_m y\\right)} dx dy $$"
   ]
  },
  {
   "cell_type": "markdown",
   "metadata": {
    "collapsed": true
   },
   "source": [
    "<h3>Simple Harmonic Oscillator</h3>\n",
    "\n",
    "$$ m \\frac{d^2 q}{d t^2} + k q = 0 $$\n",
    "\n",
    "$$ q_0 = q(0) \\qquad p_0 = m \\dot q(0) $$\n",
    "\n",
    "Has solution\n",
    "\n",
    "$$ q(t) = q_0 \\cos(\\omega t)\n",
    "  +  \\frac{\\dot q_0}{\\omega} \\sin (\\omega t) $$\n",
    "  \n",
    "$$ q(t) = q_0 \\frac{e^{i \\omega t} + e^{-i \\omega t}}{2}\n",
    "  + \\frac{\\dot q_0}{\\omega} \\frac{e^{i \\omega t} - e^{-i \\omega t}}{2 i} $$\n",
    "  \n",
    "$$ q(t) = \\frac{1}{2} \\left(q_0 + \\frac{\\dot q_0}{i \\omega} \\right) e^{i \\omega t}\n",
    "  + \\frac{1}{2} \\left(q_0 - \\frac{\\dot q_0}{i \\omega} \\right) e^{- i \\omega t} $$\n",
    "  \n",
    "$$ q(t) = \\frac{1}{2} \\left[a_0 e^{i \\omega t} + a_0^* e^{-i \\omega t} \\right] $$"
   ]
  },
  {
   "cell_type": "code",
   "execution_count": null,
   "metadata": {
    "collapsed": true
   },
   "outputs": [],
   "source": []
  }
 ],
 "metadata": {
  "kernelspec": {
   "display_name": "Python 3",
   "language": "python",
   "name": "python3"
  },
  "language_info": {
   "codemirror_mode": {
    "name": "ipython",
    "version": 3
   },
   "file_extension": ".py",
   "mimetype": "text/x-python",
   "name": "python",
   "nbconvert_exporter": "python",
   "pygments_lexer": "ipython3",
   "version": "3.6.0"
  }
 },
 "nbformat": 4,
 "nbformat_minor": 2
}
