{
 "cells": [
  {
   "cell_type": "markdown",
   "metadata": {},
   "source": [
    "### Appendix ###\n",
    "\n",
    "Let us verify the below equations with some admittedly hackey notation.\n",
    "\n",
    "First note that\n",
    "\n",
    "\\begin{gather}\n",
    "[E]_i = c F^{i 0} \\qquad\n",
    "[B]_i = -\\tfrac{1}{2} \\epsilon_{i j k} F^{j k} \\qquad\n",
    "[D]_i = \\tfrac{1}{c} P^{i 0} \\qquad\n",
    "[H]_i = -\\tfrac{1}{2} \\epsilon_{i j k} P^{j k}\n",
    "\\end{gather}\n",
    "\n",
    "and show that\n",
    "\n",
    "\\begin{gather}\n",
    "[E]_i\n",
    "= c F^{i 0}\n",
    "= c (\\partial^i A^0 - \\partial^0 A^i)\n",
    "= -c \\partial_i A^0 - c \\partial_0 A^i\n",
    "= [-\\nabla \\phi - \\partial_t A]_i\n",
    "\\end{gather}\n",
    "\n",
    "\\begin{gather}\n",
    "[B]_i\n",
    "= -\\tfrac{1}{2} \\epsilon_{i j k} F^{j k}\n",
    "= -\\tfrac{1}{2} \\epsilon_{i j k} (\\partial^j A^k - \\partial^k A^j)\\\n",
    "= \\epsilon_{i j k} \\partial_j A^k\n",
    "= [\\nabla \\times A]_i\n",
    "\\end{gather}\n",
    "\n",
    "\\begin{gather}\n",
    "[\\nabla \\cdot D]\n",
    "= \\partial_i \\tfrac{1}{c} P^{i 0}\n",
    "= \\tfrac{1}{c} \\partial_\\alpha P^{\\alpha 0}\n",
    "= \\tfrac{1}{c} J^0\n",
    "= [\\rho]\n",
    "\\end{gather}\n",
    "\n",
    "\\begin{gather}\n",
    "[-\\partial_t D + \\nabla \\times H]_i\n",
    "= -\\partial_0 P^{i 0} - \\epsilon^{i j k} \\partial_j (\\tfrac{1}{2} \\epsilon_{k m n} P^{m n})\n",
    "= -\\partial_0 P^{i 0} - \\partial_j P^{i j}\n",
    "= \\partial_\\alpha P^{\\alpha i}\n",
    "= J^i = [J]_i\n",
    "\\end{gather}\n",
    "\n",
    "\n",
    "Second note that\n",
    "\n",
    "\\begin{gather}\n",
    "\\frac{\\partial F^{\\alpha \\beta}}{\\partial [E]_i}\n",
    "= \\frac{1}{c} (\\delta^\\alpha_i \\delta^\\beta_0 - \\delta^\\alpha_0 \\delta^\\beta_i)\n",
    "\\qquad\n",
    "\\frac{\\partial F^{j k}}{\\partial [B]_i}\n",
    "= -\\epsilon^{i j k}\n",
    "\\qquad\n",
    "\\frac{\\partial A^i}{\\partial [\\phi]} = \\frac{1}{c} \\delta^i_0\n",
    "\\qquad\n",
    "\\frac{\\partial A^j}{\\partial [A]_i} = \\delta^j_i\n",
    "\\end{gather}\n",
    "\n",
    "and show that\n",
    "\n",
    "\\begin{gather}\n",
    "\\frac{\\partial \\mathcal{L}}{\\partial [E]_i}\n",
    "= \\frac{\\partial \\mathcal{L}}{\\partial F^{\\alpha \\beta}}\n",
    "\\frac{1}{c} (\\delta^\\alpha_i \\delta^\\beta_0 - \\delta^\\alpha_0 \\delta^\\beta_i)\n",
    "= \\frac{2}{c} \\frac{\\partial \\mathcal{L}}{\\partial F^{i 0}}\n",
    "= -\\frac{2}{c} \\frac{\\partial \\mathcal{L}}{\\partial F_{i 0}}\n",
    "= \\frac{1}{c} P^{i 0}\n",
    "= [D]_i\n",
    "\\\\\n",
    "\\frac{\\partial \\mathcal{L}}{\\partial [B]_i}\n",
    "= -\\frac{\\partial \\mathcal{L}}{\\partial F^{j k}} \\epsilon^{i j k}\n",
    "= -\\frac{\\partial \\mathcal{L}}{\\partial F_{j k}} \\epsilon^{i j k}\n",
    "= \\frac{1}{2} \\epsilon_{i j k} P^{j k}\n",
    "= -[H]_i\n",
    "\\\\\n",
    "\\frac{\\partial \\mathcal{L}}{\\partial [\\phi]}\n",
    "= \\frac{\\partial \\mathcal{L}}{\\partial A^i} \\frac{1}{c} \\delta^i_0\n",
    "= \\frac{1}{c} \\frac{\\partial \\mathcal{L}}{\\partial A^0}\n",
    "= -\\frac{1}{c} J^0\n",
    "= -[\\rho]\n",
    "\\\\\n",
    "\\frac{\\partial \\mathcal{L}}{\\partial [A]_i}\n",
    "= \\frac{\\partial \\mathcal{L}}{\\partial A^j} \\delta^i_j\n",
    "= \\frac{\\partial \\mathcal{L}}{\\partial A^i}\n",
    "= -\\frac{\\partial \\mathcal{L}}{\\partial A_i}\n",
    "= J^i\n",
    "= [J]_i\n",
    "\\end{gather}"
   ]
  },
  {
   "cell_type": "markdown",
   "metadata": {},
   "source": [
    "### Maxwell's Equations ###\n",
    "\n",
    "Let us define the following four-vectors and tensors.\n",
    "\n",
    "\\begin{gather}\n",
    "\\partial_\\alpha = \\begin{pmatrix} \\frac{1}{c}\\partial_t & \\partial_x & \\partial_y & \\partial_z \\end{pmatrix}\n",
    "\\qquad\n",
    "A^\\alpha = \\left( \\begin{matrix}\\frac{1}{c}\\phi & A_x & A_y & A_z \\end{matrix}\\right)\n",
    "\\qquad\n",
    "J^\\alpha = \\begin{pmatrix} c\\rho & J_x & J_y & J_z \\end{pmatrix}  \n",
    "\\end{gather}\n",
    "\n",
    "\\begin{gather}\n",
    "F^{\\alpha \\beta} = \\begin{pmatrix}\n",
    "0       & -E_x / c & -E_y / c & -E_z / c \\\\\n",
    "E_x / c &  0       & -B_z     &  B_y     \\\\\n",
    "E_y / c &  B_z     &    0     & -B_x     \\\\\n",
    "E_z / c & -B_y     &  B_x     &  0       \\end{pmatrix}\n",
    "\\qquad\n",
    "P^{\\alpha\\beta} = \\begin{pmatrix}\n",
    "0 & -c D_x & -c D_y & -c D_z \\\\\n",
    " c D_x & 0 & -H_z & H_y \\\\\n",
    " c D_y & H_z & 0 & -H_x \\\\\n",
    " c D_z & -H_y & H_x & 0\n",
    "\\end{pmatrix}\n",
    "\\end{gather}\n",
    "\n",
    "With these, Maxwell's equations can be written in a compact form.\n",
    "\n",
    "\\begin{gather}\n",
    "F^{\\alpha \\beta} = \\partial^\\alpha A^\\beta - \\partial^\\beta A^\\alpha\n",
    "\\quad \\Rightarrow \\quad\n",
    "\\begin{cases}\n",
    "E = -\\nabla \\phi - \\dfrac{\\partial A}{\\partial t} \\\\\n",
    "B = \\nabla \\times A \\vphantom{\\dfrac{\\partial A}{\\partial t}}\n",
    "\\end{cases}\n",
    "\\end{gather}\n",
    "\n",
    "The first pair of equations can be viewed as the definition of the electric and magnetic fields.  As we will see, the second pair of equations can be derived from a general Lagrangian. "
   ]
  },
  {
   "cell_type": "markdown",
   "metadata": {},
   "source": [
    "In general, we have $\\mathcal{L}(\\partial_\\alpha A_\\beta, A_\\beta)$.  This notation is a different.  The Lagrangian in not a function of $\\partial_\\alpha A_\\beta$ and $A_\\beta$ for particular values of $\\alpha$ and $\\beta$.  Rather it is a functions of all combinations of values between 0 and 3. That is, the Lagrangian is a function of twenty variables.  Minimumizing the action gives\n",
    "\n",
    "\\begin{gather}\n",
    "\\partial_\\alpha \\frac{\\partial \\mathcal{L}}{\\partial (\\partial_\\alpha A_\\beta)}\n",
    "= \\frac{\\partial \\mathcal{L}}{\\partial A_\\beta}\n",
    "\\end{gather}\n",
    "\n",
    "For the particular case where $\\mathcal{L}(F_{\\alpha\\beta}, A_\\beta)$, one can show that the previuos equation becomes\n",
    "\n",
    "\\begin{gather}\n",
    "\\partial_\\alpha 2 \\frac{\\partial \\mathcal{L}}{\\partial F_{\\alpha\\beta}}\n",
    "= \\frac{\\partial \\mathcal{L}}{\\partial A_\\beta}\n",
    "\\end{gather}\n",
    "\n",
    "With the following definitons\n",
    "\\begin{gather}\n",
    "P^{\\alpha\\beta} = -2 \\frac{\\partial \\mathcal{L}}{\\partial F_{\\alpha\\beta}}\n",
    "\\quad \\Rightarrow \\quad\n",
    "\\begin{cases}\n",
    "D = \\nabla_E \\mathcal{L} \\vphantom{\\dfrac{\\partial A}{\\partial t}} \\\\\n",
    "H = -\\nabla_B \\mathcal{L} \\vphantom{\\dfrac{\\partial A}{\\partial t}}\n",
    "\\end{cases}\n",
    "\\end{gather}\n",
    "\n",
    "\\begin{gather}\n",
    "J^\\beta = -\\frac{\\partial \\mathcal{L}}{\\partial A_\\beta}\n",
    "\\quad \\Rightarrow \\quad\n",
    "\\begin{cases}\n",
    "\\rho = - \\dfrac{\\partial \\mathcal{L}}{\\partial \\phi} \\vphantom{\\dfrac{\\partial A}{\\partial t}} \\\\\n",
    "J = \\nabla_A \\mathcal{L} \\vphantom{\\dfrac{\\partial A}{\\partial t}}\n",
    "\\end{cases}\n",
    "\\end{gather}\n",
    "\n",
    "the previous equation becomes\n",
    "\n",
    "\\begin{gather}\n",
    "\\partial_\\alpha P^{\\alpha \\beta} = J^\\beta\n",
    "\\quad \\Rightarrow \\quad\n",
    "\\begin{cases}\n",
    "\\nabla \\cdot D = \\rho \\vphantom{\\dfrac{\\partial A}{\\partial t}} \\\\\n",
    "- \\dfrac{\\partial D}{\\partial t} + \\nabla \\times H = J\n",
    "\\end{cases}\n",
    "\\end{gather}\n",
    "\n",
    "We see that the second pair of Maxwell's equations can be seen as arising from a general Lagrangian.  In general, $D$ and $H$ are complicated functions of $E$ and $B$."
   ]
  },
  {
   "cell_type": "markdown",
   "metadata": {},
   "source": [
    "### The General Energy-Momentum Tensor ###\n",
    "\n",
    "The following equation is derived in an AJP paper using Noether's theorem.  As before, we assume $\\mathcal{L}(A_\\alpha, F_{\\alpha\\beta})$ and use our previous definitions.\n",
    "\n",
    "\\begin{gather}\n",
    "\\Theta^{\\alpha}_{\\phantom\\alpha \\beta}\n",
    "= -J^\\alpha A_\\beta\n",
    "- P^{\\alpha \\gamma} F_{\\beta \\gamma} - \\delta^{\\alpha}_{\\phantom\\alpha \\beta} \\mathcal{L}\n",
    "\\end{gather}"
   ]
  },
  {
   "cell_type": "markdown",
   "metadata": {},
   "source": [
    "\\begin{split}\n",
    "\\Theta^{0 0}\n",
    "&= \\Theta^{0}_{\\phantom\\alpha 0} \\\\\n",
    "&= -J^0 A_0 - P^{0 \\gamma} F_{0 \\gamma} - \\delta^{0}_{\\phantom\\alpha 0} \\mathcal{L} \\\\\n",
    "&= -J^0 A_0 - P^{0 0} F_{0 0} - P^{0 i} F_{0 i} - \\mathcal{L} \\\\\n",
    "&= -J^0 A^0 + P^{i 0} F^{i 0} - \\mathcal{L} \\\\\n",
    "&= -\\rho \\phi + D \\cdot E - \\mathcal{L} \\\\\n",
    "\\end{split}"
   ]
  },
  {
   "cell_type": "markdown",
   "metadata": {},
   "source": [
    "\\begin{split}\n",
    "\\Theta^{0 i}\n",
    "&= -\\Theta^{0}_{\\phantom\\alpha i} \\\\\n",
    "&= J^0 A_i + P^{0 \\gamma} F_{i \\gamma} + \\delta^0_{\\phantom\\alpha i} \\mathcal{L} \\\\\n",
    "&= J^0 A_i + P^{0 0} F_{i 0} + P^{0 j} F_{i j} \\\\\n",
    "&= -J^0 A^i - P^{j 0} F^{i j} \\\\\n",
    "&= -[c \\rho] [A]_i + \\epsilon^{i j k}  c [D]_j [B]_k \\qquad \\\\\n",
    "&= [-c \\rho A + c D \\times B]_i\n",
    "\\end{split}\n",
    "\n",
    "\\begin{split}\n",
    "\\Theta^{i 0}\n",
    "&= -\\Theta^{i}_{\\phantom\\alpha 0} \\\\\n",
    "&= J^i A_0 + P^{i \\gamma} F_{0 \\gamma} + \\delta^i_{\\phantom\\alpha 0} \\mathcal{L} \\\\\n",
    "&= J^i A_0 + P^{i 0} F_{0 0} + P^{i j} F_{0 j} \\\\\n",
    "&= J^i A^0 - P^{i j} F^{0 j} \\\\\n",
    "\\end{split}"
   ]
  },
  {
   "cell_type": "markdown",
   "metadata": {},
   "source": [
    "\\begin{gather}\n",
    "F^{i 0} = \\frac{1}{c} [E]_i \\qquad\n",
    "F^{i j} = -\\epsilon^{i j k} [B]_k \\qquad\n",
    "P^{i 0} = c [D]_i \\qquad\n",
    "P^{i j} = -\\epsilon^{i j k} [H]_k \\qquad\n",
    "\\end{gather}"
   ]
  },
  {
   "cell_type": "code",
   "execution_count": null,
   "metadata": {
    "collapsed": true
   },
   "outputs": [],
   "source": []
  }
 ],
 "metadata": {
  "kernelspec": {
   "display_name": "Python 3",
   "language": "python",
   "name": "python3"
  },
  "language_info": {
   "codemirror_mode": {
    "name": "ipython",
    "version": 3
   },
   "file_extension": ".py",
   "mimetype": "text/x-python",
   "name": "python",
   "nbconvert_exporter": "python",
   "pygments_lexer": "ipython3",
   "version": "3.6.0"
  }
 },
 "nbformat": 4,
 "nbformat_minor": 2
}
